src/Bedrock/End2End/X25519/Field25519.v
@@ -1,3 +1,4 @@
+Require Import Crypto.Spec.Curve25519.
 Require Import Coq.Strings.String. Local Open Scope string_scope.
 Require Import Coq.Lists.List.
 Require Import Coq.ZArith.ZArith.
@@ -38,17 +39,8 @@ Section Field.
   Instance translation_parameters_ok : Types.ok.
   Proof using ext_spec_ok. constructor; try exact _; apply prefix_name_gen_unique. Qed.
 
-  (* Define Curve25519 field *)
-  Instance field_parameters : FieldParameters.
-  Proof using Type.
-    let M := (eval vm_compute in (Z.to_pos (UnsaturatedSolinas.m s c))) in
-    (* curve 'A' parameter *)
-    let a := constr:(F.of_Z M 486662) in
-    let prefix := constr:("fe25519_"%string) in
-    eapply
-      (field_parameters_prefixed
-         M ((a - F.of_Z _ 2) / F.of_Z _ 4)%F prefix).
-  Defined.
+  Instance field_parameters : FieldParameters :=
+    field_parameters_prefixed Curve25519.p Curve25519.M.a24 "fe25519_"%string.
 
   (* Call fiat-crypto pipeline on all field operations *)
   Instance fe25519_ops : unsaturated_solinas_ops (ext_spec:=ext_spec) n s c.
